Docs/ContextualEmbedding/package.lean
@@ -2,5 +2,6 @@ import «ContextualEmbedding».CE
 import «ContextualEmbedding».__CEFnExample
 import «ContextualEmbedding».CEEval
 import «ContextualEmbedding».Extrinsic.CE
+import «ContextualEmbedding».Extrinsic.CEEval
 import «ContextualEmbedding».CELeveledUpSTLC
 import «ContextualEmbedding».CELeveledUpLinear
